TotalConsistency.thy
@@ -3,15 +3,16 @@ imports TotalExpressions
 begin
 
 
-definition red_inhale_nset :: "program \<Rightarrow>  'a interp \<Rightarrow> ('a full_total_state \<Rightarrow> bool) \<Rightarrow> assertion \<Rightarrow> 'a full_total_state \<Rightarrow> ('a full_total_state) set"
-  where "red_inhale_nset Pr \<Delta> R A \<omega> = { \<omega>'. red_inhale Pr \<Delta> R A \<omega> (RNormal \<omega>')}"
+definition red_inhale_nset :: "'a total_context \<Rightarrow> ('a full_total_state \<Rightarrow> bool) \<Rightarrow> assertion \<Rightarrow> 'a full_total_state \<Rightarrow> ('a full_total_state) set"
+  where "red_inhale_nset ctxt R A \<omega> = { \<omega>'. red_inhale ctxt R A \<omega> (RNormal \<omega>')}"
 
-definition unfold_rel_general_set  :: "program \<Rightarrow> 'a interp \<Rightarrow> ('a full_total_state) set \<Rightarrow> ('a full_total_state) set \<Rightarrow> bool"
-  where "unfold_rel_general_set Pr \<Delta> W W' \<equiv> \<exists> pred vs q. W' = {\<omega>'. \<exists> \<omega> \<in> W. unfold_rel Pr \<Delta> pred vs q \<omega> \<omega>'}"
+definition unfold_rel_general_set  :: "'a total_context \<Rightarrow> ('a full_total_state \<Rightarrow> bool) \<Rightarrow> ('a full_total_state) set \<Rightarrow> ('a full_total_state) set \<Rightarrow> bool"
+  where "unfold_rel_general_set ctxt R W W' \<equiv> \<exists> pred vs q. W' = {\<omega>'. \<exists> \<omega> \<in> W. unfold_rel ctxt R pred vs q \<omega> \<omega>'}"
 
-definition unfold_rel_multi_set :: "program \<Rightarrow> 'a interp \<Rightarrow> ('a full_total_state) set \<Rightarrow> ('a full_total_state) set \<Rightarrow> bool"
-  where "unfold_rel_multi_set Pr \<Delta> \<equiv> rtranclp (unfold_rel_general_set Pr \<Delta>)"
+definition unfold_rel_multi_set :: "'a total_context \<Rightarrow> ('a full_total_state \<Rightarrow> bool) \<Rightarrow> ('a full_total_state) set \<Rightarrow> ('a full_total_state) set \<Rightarrow> bool"
+  where "unfold_rel_multi_set ctxt R \<equiv> rtranclp (unfold_rel_general_set ctxt R)"
 
+(*
 definition unfold_consistent_set :: "program \<Rightarrow> 'a interp \<Rightarrow> 'a full_total_state \<Rightarrow> bool"
   where "unfold_consistent_set Pr \<Delta> \<omega> \<equiv>
           \<forall> W' \<omega>' pred_id vs q. (unfold_rel_multi_set Pr \<Delta> {\<omega>} W' \<and> \<omega>' \<in> W' \<and> pgt (get_mp_total_full \<omega>' (pred_id,vs)) q) \<longrightarrow> 
@@ -25,18 +26,22 @@ proof ((rule allI)+, rule impI)
   fix W' \<omega>' pred_id vs q
   assume "unfold_rel_multi_set Pr \<Delta> {\<omega>} W' \<and> \<omega>' \<in> W' \<and> pgt (get_mp_total_full \<omega> (pred_id, vs)) q"
   oops
+*)
 
 lemma unfold_rel_general_set_non_empty:
-  assumes "unfold_rel_general_set Pr \<Delta> W W'" and "W' \<noteq> {}"
+  assumes "unfold_rel_general_set ctxt R W W'" and "W' \<noteq> {}"
   shows "W \<noteq> {}"
   using assms
   unfolding unfold_rel_general_set_def
   by blast
 
+(* This theorem is harder to prove with the corrected definition of total heap consistency that unfolds
+a full predicate at each step.
+
 lemma unfolding_consistent_1: 
-  assumes "unfold_rel_multi_set Pr \<Delta> W1 W2" and "W1 \<noteq> {}" and 
-          "\<forall> \<omega> \<in> W1. unfold_consistent Pr \<Delta> \<omega>" and "W2 \<noteq> {}"
-  shows "\<exists>\<omega>' \<in> W2. unfold_consistent Pr \<Delta> \<omega>'"
+  assumes "unfold_rel_multi_set ctxt R W1 W2" and "W1 \<noteq> {}" and 
+          "\<forall> \<omega> \<in> W1. total_heap_consistent ctxt \<omega>" and "W2 \<noteq> {}"
+  shows "\<exists>\<omega>' \<in> W2. total_heap_consistent ctxt \<omega>'"
   using assms
   unfolding unfold_rel_multi_set_def
 proof (induction rule: rtranclp_induct)
@@ -44,22 +49,16 @@ case base
   thus ?case by blast
 next
   case (step W2 W3)
-  from this obtain \<omega>2 where "\<omega>2 \<in> W2" and \<omega>2_cons:"unfold_consistent Pr \<Delta> \<omega>2" using unfold_rel_general_set_non_empty by blast
-  from step(2) obtain pred_id vs q where "W3 = {\<omega>'. \<exists> \<omega> \<in> W2. unfold_rel Pr \<Delta> pred_id vs q \<omega> \<omega>'}"
+  from this obtain \<omega>2 where "\<omega>2 \<in> W2" and \<omega>2_cons:"total_heap_consistent ctxt \<omega>2" using unfold_rel_general_set_non_empty by blast
+  from step(2) obtain pred_id vs q where "W3 = {\<omega>'. \<exists> \<omega> \<in> W2. unfold_rel ctxt R pred_id vs q \<omega> \<omega>'}"
     unfolding unfold_rel_general_set_def by blast
   with \<open>W3 \<noteq> {}\<close> and \<open>\<omega>2 \<in> W2\<close> have "pgt (get_mp_total_full \<omega>2 (pred_id,vs)) q"
     
-  thm unfold_consistent.cases
+    
   from \<omega>2_cons obtain \<omega>3 where "unfold_rel Pr \<Delta> pred vs q \<omega>2 \<omega>3"
-    apply (cases rule: unfold_consistent.cases)
+    apply (cases rule: total_heap_consistent.cases)
   then show ?case    
 qed
-
-
-
-
-                                       
-
-
+*)
 
 end
