TotalExpressions.thy
@@ -1,10 +1,11 @@
-section \<open>Expression evaluation, inhale, total heap consistency\<close>
+section \<open>Expression evaluation, well-definedness, inhale, total heap consistency\<close>
 
 theory TotalExpressions
 imports Viper.ViperLang Viper.ValueAndBasicState TotalViperState Viper.Binop Viper.DeBruijn Viper.PredicatesUtil TotalUtil
 begin
 
 subsection \<open>Heap-dependent function interpretation\<close>
+
 type_synonym 'a heapfun_repr = "'a val list \<Rightarrow> 'a full_total_state \<rightharpoonup> 'a extended_val"
 type_synonym 'a interp = "function_ident \<rightharpoonup> 'a heapfun_repr"
 
@@ -17,13 +18,18 @@ for \<^term>\<open>(f::'a heapfun_repr) vs \<omega>\<close> are
 \<^item> \<^term>\<open>Some (Val v)\<close>: There is no typing issue and the function call is well-defined. The resulting value is \<^term>\<open>v\<close>.
 \<close>
 
-subsection \<open>Pure expression evaluation and inhale\<close>
+subsection\<open>Evaluation of pure expressions, well-definedness of pure expressions, inhale of assertions\<close>
 
 datatype 'a standard_result = RMagic | RFailure | RNormal "'a full_total_state"
 
 definition get_valid_locs :: "'a full_total_state \<Rightarrow> heap_loc set"
   where "get_valid_locs \<omega> = {lh |lh. pgt (get_mh_total_full \<omega> lh) pnone}"
 
+
+text \<open>Construct the set of states that can be reached after an inhaling field permission.
+      \<^term>\<open>R\<close> expresses when a state is consistent. If \<^term>\<open>p_opt = Some q\<close> then precisely \<^term>\<open>q\<close> 
+      permission is added and otherwise there are no explicit constraints on the added permission
+      (useful to model adding wildcard permission).\<close>
 
 definition inhale_perm_single :: "('a full_total_state \<Rightarrow> bool) \<Rightarrow> 'a full_total_state \<Rightarrow> heap_loc \<Rightarrow> prat option \<Rightarrow> 'a full_total_state set"
   where "inhale_perm_single R \<omega> lh p_opt =
@@ -32,6 +38,8 @@ definition inhale_perm_single :: "('a full_total_state \<Rightarrow> bool) \<Rig
                pgte pwrite (padd (get_mh_total_full \<omega> lh) q) \<and>
                \<omega>' = update_mh_total_full \<omega> ((get_mh_total_full \<omega>)(lh := (padd (get_mh_total_full \<omega> lh) q)))
        }"
+
+text \<open>Construct the set of states that can be reached after an inhaling predicate permission.\<close>
 
 definition inhale_perm_single_pred :: "('a full_total_state \<Rightarrow> bool) \<Rightarrow> 'a full_total_state \<Rightarrow> 'a predicate_loc \<Rightarrow> prat option \<Rightarrow> 'a full_total_state set"
   where "inhale_perm_single_pred R \<omega> lp p_opt = 
@@ -46,6 +54,12 @@ inductive th_result_rel :: "bool \<Rightarrow> bool \<Rightarrow> ('a full_total
 | THResultMagic: "th_result_rel True False W RMagic"
 | THResultFailure: "th_result_rel False b W RFailure"
 
+text \<open>\<^const>\<open>th_result_rel\<close> is an auxiliary relation. \<^term>\<open>th_result_rel bFailure bMagic W res\<close> is 
+used in the following way:
+  \<^item> \<^term>\<open>bFailure\<close> expresses a condition that must hold for \<^term>\<open>res\<close> not to be failing state 
+  \<^item> \<^term>\<open>bMagic\<close> expresses a condition that must hold for \<^term>\<open>res\<close> not to be magic state
+  \<^item> W expresses the set of possible normal states for \<^term>\<open>res\<close>
+\<close>
 
 inductive_cases THResultNormal_case: "th_result_rel True True W (RNormal \<omega>)"
 
@@ -71,7 +85,7 @@ lemma th_result_rel_magic:
   by (cases) auto
 
 text \<open>To handle propagation of failure: If one sub_pure_exp fails, then the whole expression fails.
-This definition is almost identical to a similar definition in more abstract Viper semantics.
+This definition is almost identical to a similar definition in a more abstract Viper semantics.
 One potential difference is that here the body of an \<^const>\<open>Unfolding\<close> expression is not a 
 subexpression, since the well-definedness of a corresponding body must be evaluated in a separate 
 state.\<close>
@@ -99,217 +113,200 @@ fun sub_expressions_atomic :: "pure_exp atomic_assert \<Rightarrow> pure_exp set
 | "sub_expressions_atomic (Acc x f p) = {x} \<union> sub_expressions_exp_or_wildcard p"
 | "sub_expressions_atomic (AccPredicate P exps p) = set exps \<union> sub_expressions_exp_or_wildcard p"
 
-text\<open>Pure expression evaluation, where the set of heap locations expresses the set of readable locations
-(if no set is provided, then all locations can be read).
-\<close>
-
 record 'a total_context =
+  program_total :: program
   fun_interp_total :: "'a interp"
   absval_interp_total :: "'a \<Rightarrow> abs_type"
 
-inductive red_pure_exp_total :: "program \<Rightarrow> 'a total_context \<Rightarrow> 'a full_total_state option \<Rightarrow> pure_exp \<Rightarrow> 'a full_total_state \<Rightarrow> 'a extended_val \<Rightarrow> bool"
+
+text \<open>Expression evaluation, well-definedness of expressions and inhale are defined in a mutually
+inductive way. The reason is that well-definedness uses inhale to express well-definedness of 
+unfolding expressions and inhale fails if some subexpression is not well-defined. Expression evaluation
+itself without well-definedness checks could be defined independently. However, since expression evaluation
+and well-definedness follow similar rules for many connectives, we decided to express them in the same
+relation, where one uses one of the parameters to distinguish expression evaluation from well-definedness.
+
+Expression evaluation either results in a value or in a failure. Failure occurs if some operation is 
+not defined (e.g., division by 0, null dereference,...). Importantly, expression evaluation is defined
+for all field accesses (with a non-null receiver), since the heap is total. 
+Well-definedness is defined the same as expression evaluation, except that failure also occurs if
+a field is accesses for which no permission is held in the mask.
+
+All three relations (evaluation, well-definedness, inhale) take a unary relation \<^term>\<open>R\<close> on states 
+as input.This relation represents when a state is consistent. Inhale progresses after adding new permission only 
+if the resulting state is consistent.
+\<close>
+
+inductive red_pure_exp_total :: "'a total_context \<Rightarrow> ('a full_total_state \<Rightarrow> bool) \<Rightarrow> 'a full_total_state option \<Rightarrow> pure_exp \<Rightarrow> 'a full_total_state \<Rightarrow> 'a extended_val \<Rightarrow> bool"
   ("_, _, _ \<turnstile> ((\<langle>_;_\<rangle>) [\<Down>]\<^sub>t _)" [51,51,51,0,51,51] 81) and
-   red_pure_exps_total :: "program \<Rightarrow> 'a total_context \<Rightarrow> 'a full_total_state option \<Rightarrow> pure_exp list \<Rightarrow> 'a full_total_state \<Rightarrow> (('a val) list) option \<Rightarrow> bool" and
-   red_inhale :: "program \<Rightarrow>  'a total_context \<Rightarrow> ('a full_total_state \<Rightarrow> bool) \<Rightarrow> assertion \<Rightarrow> 'a full_total_state \<Rightarrow> 'a standard_result \<Rightarrow> bool" and
-   unfold_rel :: "program \<Rightarrow> 'a total_context \<Rightarrow> predicate_ident \<Rightarrow> ('a val list) \<Rightarrow> prat \<Rightarrow> 'a full_total_state \<Rightarrow> 'a full_total_state \<Rightarrow> bool"
-  for Pr :: program and ctxt :: "'a total_context"
+   red_pure_exps_total :: "'a total_context \<Rightarrow>  ('a full_total_state \<Rightarrow> bool) \<Rightarrow> 'a full_total_state option \<Rightarrow> pure_exp list \<Rightarrow> 'a full_total_state \<Rightarrow> (('a val) list) option \<Rightarrow> bool" and
+   red_inhale :: "'a total_context \<Rightarrow> ('a full_total_state \<Rightarrow> bool) \<Rightarrow> assertion \<Rightarrow> 'a full_total_state \<Rightarrow> 'a standard_result \<Rightarrow> bool" and
+   unfold_rel :: "'a total_context \<Rightarrow> ('a full_total_state \<Rightarrow> bool) \<Rightarrow> predicate_ident \<Rightarrow> ('a val list) \<Rightarrow> prat \<Rightarrow> 'a full_total_state \<Rightarrow> 'a full_total_state \<Rightarrow> bool"
+  for ctxt :: "'a total_context" and R :: "'a full_total_state \<Rightarrow> bool"
   where
 \<comment>\<open>unfold_rel\<close>
+
   UnfoldRelStep: 
-    "\<lbrakk> ViperLang.predicates Pr pred_id = Some pred_decl;
+    "\<lbrakk> ViperLang.predicates (program_total ctxt) pred_id = Some pred_decl;
      ViperLang.predicate_decl.body pred_decl = Some pred_body;
      m = get_mp_total_full \<omega>;
      pgte (m (pred_id,vs)) q;
      q \<noteq> pnone;
-     m' = m( (pred_id,vs) := psub (m (pred_id, vs)) q);
+     m' = m( (pred_id,vs) := psub (m (pred_id, vs)) q );
      \<omega>2 = (nth_option vs, get_trace_total \<omega>, update_mp_total (get_total_full \<omega>) m');
-     red_inhale Pr ctxt (\<lambda>_. True) (syntactic_mult (Rep_prat q) pred_body) \<omega>2 (RNormal \<omega>') \<rbrakk> \<Longrightarrow> 
-     unfold_rel Pr ctxt pred_id vs q \<omega> \<omega>'"
+     red_inhale ctxt R (syntactic_mult (Rep_prat q) pred_body) \<omega>2 (RNormal \<omega>') \<rbrakk> \<Longrightarrow> 
+     unfold_rel ctxt R pred_id vs q \<omega> \<omega>'"
 
 \<comment>\<open>Atomic inhale\<close>
 | InhAcc: 
-    "\<lbrakk> Pr, ctxt, Some \<omega> \<turnstile> \<langle>e_r; \<omega>\<rangle> [\<Down>]\<^sub>t Val (VRef r); 
-       Pr, ctxt, Some \<omega> \<turnstile> \<langle>e_p; \<omega>\<rangle> [\<Down>]\<^sub>t Val (VPerm p); 
+    "\<lbrakk> ctxt, R, Some \<omega> \<turnstile> \<langle>e_r; \<omega>\<rangle> [\<Down>]\<^sub>t Val (VRef r); 
+       ctxt, R, Some \<omega> \<turnstile> \<langle>e_p; \<omega>\<rangle> [\<Down>]\<^sub>t Val (VPerm p); 
        W' = inhale_perm_single R \<omega> (the_address r,f) (Some (Abs_prat p));
        th_result_rel (p \<ge> 0) (W' \<noteq> {} \<and> r \<noteq> Null) W' res \<rbrakk> \<Longrightarrow>
-       red_inhale Pr ctxt R (Atomic (Acc e_r f (PureExp e_p))) \<omega> res"
+       red_inhale ctxt R (Atomic (Acc e_r f (PureExp e_p))) \<omega> res"
 | InhAccPred:
-    "\<lbrakk> Pr, ctxt, Some \<omega> \<turnstile> \<langle>e_p; \<omega>\<rangle> [\<Down>]\<^sub>t Val (VPerm p);
-       red_pure_exps_total Pr ctxt (Some \<omega>) e_args \<omega> (Some v_args);
+    "\<lbrakk> ctxt, R, Some \<omega> \<turnstile> \<langle>e_p; \<omega>\<rangle> [\<Down>]\<^sub>t Val (VPerm p);
+       red_pure_exps_total ctxt R (Some \<omega>) e_args \<omega> (Some v_args);
        W' = inhale_perm_single_pred R \<omega> (pred_id, v_args) (Some (Abs_prat p));
        th_result_rel (p \<ge> 0) (W' \<noteq> {}) W' res \<rbrakk> \<Longrightarrow>       
-       red_inhale Pr ctxt R (Atomic (AccPredicate pred_id e_args (PureExp e_p))) \<omega> res"
+       red_inhale ctxt R (Atomic (AccPredicate pred_id e_args (PureExp e_p))) \<omega> res"
 | InhAccWildcard: 
-    "\<lbrakk> Pr, ctxt, Some \<omega> \<turnstile> \<langle>e_r; \<omega>\<rangle> [\<Down>]\<^sub>t Val (VRef r);
+    "\<lbrakk> ctxt, R, Some \<omega> \<turnstile> \<langle>e_r; \<omega>\<rangle> [\<Down>]\<^sub>t Val (VRef r);
        W' = inhale_perm_single R \<omega> (the_address r,f) None;
        th_result_rel True (W' \<noteq> {} \<and> r \<noteq> Null) W' res \<rbrakk> \<Longrightarrow>
-       red_inhale Pr ctxt R (Atomic (Acc e_r f Wildcard)) \<omega> res"
+       red_inhale ctxt R (Atomic (Acc e_r f Wildcard)) \<omega> res"
 | InhAccPredWildcard: 
-    "\<lbrakk> red_pure_exps_total Pr ctxt (Some \<omega>) e_args \<omega> (Some v_args);
+    "\<lbrakk> red_pure_exps_total ctxt R (Some \<omega>) e_args \<omega> (Some v_args);
        W' = inhale_perm_single_pred R \<omega> (pred_id, v_args) None;
        th_result_rel True (W' \<noteq> {}) W' res \<rbrakk> \<Longrightarrow>
-       red_inhale Pr ctxt R (Atomic (AccPredicate pred_id e_args Wildcard)) \<omega> res"
+       red_inhale ctxt R (Atomic (AccPredicate pred_id e_args Wildcard)) \<omega> res"
 | InhPureNormalMagic: 
-    "\<lbrakk> Pr, ctxt, Some \<omega> \<turnstile> \<langle>e; \<omega>\<rangle> [\<Down>]\<^sub>t Val (VBool b) \<rbrakk> \<Longrightarrow>
-      red_inhale Pr ctxt R (Atomic (Pure e)) \<omega> (if b then RNormal \<omega> else RMagic)"
+    "\<lbrakk> ctxt, R, Some \<omega> \<turnstile> \<langle>e; \<omega>\<rangle> [\<Down>]\<^sub>t Val (VBool b) \<rbrakk> \<Longrightarrow>
+      red_inhale ctxt R (Atomic (Pure e)) \<omega> (if b then RNormal \<omega> else RMagic)"
 | InhSubFailure: 
-    "\<lbrakk> e \<in> sub_expressions_atomic A; Pr, ctxt, Some \<omega> \<turnstile> \<langle>e; \<omega>\<rangle> [\<Down>]\<^sub>t VFailure \<rbrakk> \<Longrightarrow> 
-      red_inhale Pr ctxt R (Atomic A) \<omega> RFailure"
+    "\<lbrakk> e \<in> sub_expressions_atomic A; ctxt, R, Some \<omega> \<turnstile> \<langle>e; \<omega>\<rangle> [\<Down>]\<^sub>t VFailure \<rbrakk> \<Longrightarrow> 
+      red_inhale ctxt R (Atomic A) \<omega> RFailure"
 
 \<comment>\<open>Connectives inhale\<close>
 | InhSepNormal: 
-   "\<lbrakk> red_inhale Pr ctxt R A \<omega> (RNormal \<omega>''); 
-      red_inhale Pr ctxt R B \<omega>'' res\<rbrakk> \<Longrightarrow>
-      red_inhale Pr ctxt R (A && B) \<omega> res"
+   "\<lbrakk> red_inhale ctxt R A \<omega> (RNormal \<omega>''); 
+      red_inhale ctxt R B \<omega>'' res\<rbrakk> \<Longrightarrow>
+      red_inhale ctxt R (A && B) \<omega> res"
 | InhSepFailureMagic:
-   "\<lbrakk> red_inhale Pr ctxt R A \<omega> resA; 
+   "\<lbrakk> red_inhale ctxt R A \<omega> resA; 
       resA = RFailure \<or> resA = RMagic \<rbrakk> \<Longrightarrow>
-      red_inhale Pr ctxt R (A && B) \<omega> resA"
+      red_inhale ctxt R (A && B) \<omega> resA"
 | InhImpTrue:
- "\<lbrakk> 
-    Pr, ctxt, Some \<omega> \<turnstile> \<langle>e; \<omega>\<rangle> [\<Down>]\<^sub>t (Val (VBool True)); 
-    red_inhale Pr ctxt R A \<omega> res \<rbrakk> \<Longrightarrow>
-    red_inhale Pr ctxt R (Imp e A) \<omega> res"
+ "\<lbrakk> ctxt, R, Some \<omega> \<turnstile> \<langle>e; \<omega>\<rangle> [\<Down>]\<^sub>t (Val (VBool True)); 
+    red_inhale ctxt R A \<omega> res \<rbrakk> \<Longrightarrow>
+    red_inhale ctxt R (Imp e A) \<omega> res"
 | InhImpFalse:
- "\<lbrakk> Pr, ctxt, Some \<omega> \<turnstile> \<langle>e; \<omega>\<rangle> [\<Down>]\<^sub>t Val (VBool False) \<rbrakk> \<Longrightarrow> 
-    red_inhale Pr ctxt R (Imp e A) \<omega> (RNormal \<omega>)"
+ "\<lbrakk> ctxt, R, Some \<omega> \<turnstile> \<langle>e; \<omega>\<rangle> [\<Down>]\<^sub>t Val (VBool False) \<rbrakk> \<Longrightarrow> 
+    red_inhale ctxt R (Imp e A) \<omega> (RNormal \<omega>)"
 | InhImpFailure:
- "\<lbrakk> Pr, ctxt, Some \<omega> \<turnstile> \<langle>e; \<omega>\<rangle> [\<Down>]\<^sub>t VFailure \<rbrakk> \<Longrightarrow>
-   red_inhale Pr ctxt R (Imp e A) \<omega> RFailure"
+ "\<lbrakk> ctxt, R, Some \<omega> \<turnstile> \<langle>e; \<omega>\<rangle> [\<Down>]\<^sub>t VFailure \<rbrakk> \<Longrightarrow>
+   red_inhale ctxt R (Imp e A) \<omega> RFailure"
 
-(* QP inhale rules (ignore for now)
-\<comment>\<open>QP inhale\<close>
-
-| InhQP:
- "\<lbrakk>  \<And>v. v \<in> set_from_type placeholder ty \<Longrightarrow> Pr, ctxt, Some (shift_and_add_state \<omega> v) \<turnstile> \<langle>e_r; shift_and_add_state \<omega> v\<rangle> [\<Down>]\<^sub>t (Val (VRef (Address (q1 v))));
-    \<And>v. v \<in> set_from_type placeholder ty \<Longrightarrow> Pr, ctxt, Some (shift_and_add_state \<omega> v) \<turnstile> \<langle>e_p; shift_and_add_state \<omega> v\<rangle> [\<Down>]\<^sub>t (Val (VPerm (q2 v)));
-    \<And>v. v \<in> set_from_type placeholder ty \<Longrightarrow> Pr, ctxt, Some (shift_and_add_state \<omega> v) \<turnstile> \<langle>cond; shift_and_add_state \<omega> v\<rangle> [\<Down>]\<^sub>t (Val (VBool (q3 v)));
-    m = get_mh_total_full \<omega>;
-    inj_on q2 {v. v \<in> (set_from_type placeholder ty) \<and> q3 v \<and> q2 v > 0 } ;
-   \<And>v. v \<in> set_from_type placeholder ty \<Longrightarrow> m' ((q1 v), f) = (if (q3 v) \<and> (q2 v > 0) then padd (m ((q1 v), f)) (Abs_prat (q2 v)) else m ((q1 v), f));
-   \<And>v. v \<notin> set_from_type placeholder ty \<Longrightarrow> m' ((q1 v), f) = m ((q1 v, f))
- \<rbrakk> \<Longrightarrow>
-   red_inhale Pr ctxt R (ForAll ty (Imp cond (Atomic (Acc e_r f (PureExp e_p))))) \<omega> (RNormal \<omega>')"
-
-| InhQPFailure:
- "\<lbrakk>  v \<in> set_from_type placeholder ty;
-     red_inhale Pr ctxt R (Imp cond (Atomic (Acc e_r f (PureExp e_p)))) (shift_and_add_state \<omega> v) RFailure
- \<rbrakk> \<Longrightarrow>
-   red_inhale Pr ctxt R (ForAll ty (Imp cond (Atomic (Acc e_r f (PureExp e_p))))) \<omega> RFailure"
-*)
-
-\<comment>\<open>Pure expression evaluation\<close>
+\<comment>\<open>Pure expression evaluation and well-definedness of pure expressions\<close>
 
 \<comment>\<open>List of expressions\<close>
 | RedExpList: 
-  "\<lbrakk> list_all2 (\<lambda>e v. red_pure_exp_total Pr ctxt LH e \<omega> (Val v)) es vs \<rbrakk> \<Longrightarrow>
-     red_pure_exps_total Pr ctxt LH es \<omega> (Some vs)"
+  "\<lbrakk> list_all2 (\<lambda>e v. red_pure_exp_total ctxt R \<omega>_def e \<omega> (Val v)) es vs \<rbrakk> \<Longrightarrow>
+     red_pure_exps_total ctxt R \<omega>_def es \<omega> (Some vs)"
 
 \<comment>\<open>Atomic expressions\<close>
-| RedLit: "Pr, ctxt, \<omega>_def \<turnstile> \<langle>ELit l; _\<rangle> [\<Down>]\<^sub>t Val (val_of_lit l)"
-| RedVar: "\<lbrakk> (get_store_total \<omega>) n = Some v \<rbrakk> \<Longrightarrow> Pr, ctxt, \<omega>_def \<turnstile> \<langle>Var n; \<omega>\<rangle> [\<Down>]\<^sub>t Val v"
-| RedResult: "\<lbrakk> \<sigma> 0 = Some v \<rbrakk> \<Longrightarrow> Pr, ctxt, \<omega>_def \<turnstile> \<langle>Result; (\<sigma>, _, _)\<rangle> [\<Down>]\<^sub>t Val v"
+| RedLit: "ctxt, R, \<omega>_def \<turnstile> \<langle>ELit l; _\<rangle> [\<Down>]\<^sub>t Val (val_of_lit l)"
+| RedVar: "\<lbrakk> (get_store_total \<omega>) n = Some v \<rbrakk> \<Longrightarrow> ctxt, R, \<omega>_def \<turnstile> \<langle>Var n; \<omega>\<rangle> [\<Down>]\<^sub>t Val v"
+| RedResult: "\<lbrakk> \<sigma> 0 = Some v \<rbrakk> \<Longrightarrow> ctxt, R, \<omega>_def \<turnstile> \<langle>Result; (\<sigma>, _, _)\<rangle> [\<Down>]\<^sub>t Val v"
 
 \<comment>\<open>Binop and Unop\<close>
-| RedBinopLazy: "\<lbrakk> Pr, ctxt, \<omega>_def \<turnstile> \<langle>e1; \<omega>\<rangle> [\<Down>]\<^sub>t Val v1 ; eval_binop_lazy v1 bop = Some v \<rbrakk>
-  \<Longrightarrow> Pr, ctxt, \<omega>_def \<turnstile> \<langle>Binop e1 bop e2; \<omega>\<rangle> [\<Down>]\<^sub>t Val v"                                                                        
-| RedBinop: "\<lbrakk> Pr, ctxt, \<omega>_def \<turnstile> \<langle>e1; \<omega>\<rangle> [\<Down>]\<^sub>t Val v1 ; 
-               Pr, ctxt, \<omega>_def \<turnstile> \<langle>e2; \<omega>\<rangle> [\<Down>]\<^sub>t Val v2 ; 
-               eval_binop_lazy v1 bop = None; 
-               eval_binop v1 bop v2 = BinopNormal v \<rbrakk>
-  \<Longrightarrow> Pr, ctxt, \<omega>_def \<turnstile> \<langle>Binop e1 bop e2; \<omega>\<rangle> [\<Down>]\<^sub>t Val v"
+| RedBinopLazy: 
+  "\<lbrakk> ctxt, R, \<omega>_def \<turnstile> \<langle>e1; \<omega>\<rangle> [\<Down>]\<^sub>t Val v1 ; eval_binop_lazy v1 bop = Some v \<rbrakk>\<Longrightarrow> 
+    ctxt, R, \<omega>_def \<turnstile> \<langle>Binop e1 bop e2; \<omega>\<rangle> [\<Down>]\<^sub>t Val v"                                                                        
+| RedBinop: 
+  "\<lbrakk> ctxt, R, \<omega>_def \<turnstile> \<langle>e1; \<omega>\<rangle> [\<Down>]\<^sub>t Val v1 ; 
+     ctxt, R, \<omega>_def \<turnstile> \<langle>e2; \<omega>\<rangle> [\<Down>]\<^sub>t Val v2 ; 
+     eval_binop_lazy v1 bop = None; 
+     eval_binop v1 bop v2 = BinopNormal v \<rbrakk> \<Longrightarrow> 
+  ctxt, R, \<omega>_def \<turnstile> \<langle>Binop e1 bop e2; \<omega>\<rangle> [\<Down>]\<^sub>t Val v"
 | RedBinopRightFailure: 
-      "\<lbrakk> Pr, ctxt, \<omega>_def \<turnstile> \<langle>e1; \<omega>\<rangle> [\<Down>]\<^sub>t Val v1; 
-         Pr, ctxt, \<omega>_def \<turnstile> \<langle>e2; \<omega>\<rangle> [\<Down>]\<^sub>t VFailure; 
-         eval_binop_lazy v1 bop = None;
-         \<comment>\<open>The following premise makes sure in this case that the binary operation does not reduce if
-           e1 evaluates to a value that renders the binary operation ill-typed\<close>
-         (\<exists> v2. eval_binop v1 bop v2 \<noteq> BinopTypeFailure) \<rbrakk>
-  \<Longrightarrow> Pr, ctxt, \<omega>_def \<turnstile> \<langle>Binop e1 bop e2; \<omega>\<rangle> [\<Down>]\<^sub>t VFailure"
-| RedBinopOpFailure: "\<lbrakk> Pr, ctxt, \<omega>_def \<turnstile> \<langle>e1; \<omega>\<rangle> [\<Down>]\<^sub>t Val v1 ; Pr, ctxt, \<omega>_def \<turnstile> \<langle>e2; \<omega>\<rangle> [\<Down>]\<^sub>t Val v2 ; eval_binop v1 bop v2 = BinopOpFailure ; eval_binop_lazy v1 bop = None \<rbrakk>
-  \<Longrightarrow> Pr, ctxt, \<omega>_def \<turnstile> \<langle>Binop e1 bop e2; \<omega>\<rangle> [\<Down>]\<^sub>t VFailure" (* Division by 0 *)
+  "\<lbrakk> ctxt, R, \<omega>_def \<turnstile> \<langle>e1; \<omega>\<rangle> [\<Down>]\<^sub>t Val v1; 
+     ctxt, R, \<omega>_def \<turnstile> \<langle>e2; \<omega>\<rangle> [\<Down>]\<^sub>t VFailure; 
+     eval_binop_lazy v1 bop = None;
+     \<comment>\<open>The following premise makes sure in this case that the binary operation does not reduce if
+       e1 evaluates to a value that renders the binary operation ill-typed\<close>
+     (\<exists> v2. eval_binop v1 bop v2 \<noteq> BinopTypeFailure)\<rbrakk> \<Longrightarrow> 
+   ctxt, R, \<omega>_def \<turnstile> \<langle>Binop e1 bop e2; \<omega>\<rangle> [\<Down>]\<^sub>t VFailure"
+| RedBinopOpFailure: 
+  "\<lbrakk> ctxt, R, \<omega>_def \<turnstile> \<langle>e1; \<omega>\<rangle> [\<Down>]\<^sub>t Val v1; 
+     ctxt, R, \<omega>_def \<turnstile> \<langle>e2; \<omega>\<rangle> [\<Down>]\<^sub>t Val v2; 
+     eval_binop v1 bop v2 = BinopOpFailure; 
+     eval_binop_lazy v1 bop = None \<rbrakk> \<Longrightarrow> 
+  ctxt, R, \<omega>_def \<turnstile> \<langle>Binop e1 bop e2; \<omega>\<rangle> [\<Down>]\<^sub>t VFailure" \<comment>\<open>happens for division by 0, modulo 0\<close>
 
-| RedUnop: "\<lbrakk> Pr, ctxt, \<omega>_def \<turnstile> \<langle>e; \<omega>\<rangle> [\<Down>]\<^sub>t Val v; eval_unop unop v = BinopNormal v' \<rbrakk> \<Longrightarrow> Pr, ctxt, \<omega>_def \<turnstile> \<langle>Unop unop e; \<omega>\<rangle> [\<Down>]\<^sub>t Val v'"
+| RedUnop: 
+  "\<lbrakk> ctxt, R, \<omega>_def \<turnstile> \<langle>e; \<omega>\<rangle> [\<Down>]\<^sub>t Val v; 
+     eval_unop unop v = BinopNormal v' \<rbrakk> \<Longrightarrow> 
+  ctxt, R, \<omega>_def \<turnstile> \<langle>Unop unop e; \<omega>\<rangle> [\<Down>]\<^sub>t Val v'"
 
 \<comment>\<open>Cond\<close>
-| RedCondExpTrue: "\<lbrakk> Pr, ctxt, \<omega>_def \<turnstile> \<langle>e1; \<omega>\<rangle> [\<Down>]\<^sub>t Val (VBool True) ; Pr, ctxt, \<omega>_def \<turnstile> \<langle>e2; \<omega>\<rangle> [\<Down>]\<^sub>t r \<rbrakk>
-  \<Longrightarrow> Pr, ctxt, \<omega>_def \<turnstile> \<langle>CondExp e1 e2 e3; \<omega>\<rangle> [\<Down>]\<^sub>t r"
-| RedCondExpFalse: "\<lbrakk> Pr, ctxt, \<omega>_def \<turnstile> \<langle>e1; \<omega>\<rangle> [\<Down>]\<^sub>t Val (VBool False) ; Pr, ctxt, \<omega>_def \<turnstile> \<langle>e3; \<omega>\<rangle> [\<Down>]\<^sub>t r \<rbrakk>
-  \<Longrightarrow> Pr, ctxt, \<omega>_def \<turnstile> \<langle>CondExp e1 e2 e3; \<omega>\<rangle> [\<Down>]\<^sub>t r"
+| RedCondExpTrue: 
+  "\<lbrakk> ctxt, R, \<omega>_def \<turnstile> \<langle>e1; \<omega>\<rangle> [\<Down>]\<^sub>t Val (VBool True) ; 
+    ctxt, R, \<omega>_def \<turnstile> \<langle>e2; \<omega>\<rangle> [\<Down>]\<^sub>t r \<rbrakk> \<Longrightarrow> 
+    ctxt, R, \<omega>_def \<turnstile> \<langle>CondExp e1 e2 e3; \<omega>\<rangle> [\<Down>]\<^sub>t r"
+| RedCondExpFalse: 
+  "\<lbrakk> ctxt, R, \<omega>_def \<turnstile> \<langle>e1; \<omega>\<rangle> [\<Down>]\<^sub>t Val (VBool False) ; 
+     ctxt, R, \<omega>_def \<turnstile> \<langle>e3; \<omega>\<rangle> [\<Down>]\<^sub>t r \<rbrakk> \<Longrightarrow> 
+   ctxt, R, \<omega>_def \<turnstile> \<langle>CondExp e1 e2 e3; \<omega>\<rangle> [\<Down>]\<^sub>t r"
 
 \<comment>\<open>Old\<close>
-| RedOld: "\<lbrakk> t l = Some \<phi> ; Pr, ctxt, \<omega>_def \<turnstile> \<langle>e; (\<sigma>, t, \<phi>)\<rangle> [\<Down>]\<^sub>t v \<rbrakk> \<Longrightarrow> Pr, ctxt, \<omega>_def \<turnstile> \<langle>Old l e; (\<sigma>, t, _)\<rangle> [\<Down>]\<^sub>t v"
-| RedOldFailure: "\<lbrakk> t l = None \<rbrakk> \<Longrightarrow> Pr, ctxt, \<omega>_def \<turnstile> \<langle>Old l e ; (_, t, _)\<rangle> [\<Down>]\<^sub>t VFailure" 
+| RedOld: 
+   "\<lbrakk> t l = Some \<phi> ; 
+     ctxt, R, \<omega>_def \<turnstile> \<langle>e; (\<sigma>, t, \<phi>)\<rangle> [\<Down>]\<^sub>t v \<rbrakk> \<Longrightarrow> 
+     ctxt, R, \<omega>_def \<turnstile> \<langle>Old l e; (\<sigma>, t, _)\<rangle> [\<Down>]\<^sub>t v"
+ | RedOldFailure: 
+   "\<lbrakk> t l = None \<rbrakk> \<Longrightarrow> 
+    ctxt, R, \<omega>_def \<turnstile> \<langle>Old l e ; (_, t, _)\<rangle> [\<Down>]\<^sub>t VFailure" 
 
 \<comment>\<open>Heap lookup\<close>
-| RedField: "\<lbrakk> Pr, ctxt, \<omega>_def \<turnstile> \<langle>e; \<omega>\<rangle> [\<Down>]\<^sub>t Val (VRef (Address a)) ; 
-              get_hh_total_full \<omega> (a, f) = v \<rbrakk> \<Longrightarrow> 
-       Pr, ctxt, \<omega>_def \<turnstile> \<langle>FieldAcc e f; \<omega>\<rangle> [\<Down>]\<^sub>t (if (if_Some (\<lambda>res. (a,f) \<in> get_valid_locs res) \<omega>_def) then Val v else VFailure)"
+| RedField: 
+   "\<lbrakk> ctxt, R, \<omega>_def \<turnstile> \<langle>e; \<omega>\<rangle> [\<Down>]\<^sub>t Val (VRef (Address a)); 
+      get_hh_total_full \<omega> (a, f) = v \<rbrakk> \<Longrightarrow> 
+      ctxt, R, \<omega>_def \<turnstile> \<langle>FieldAcc e f; \<omega>\<rangle> [\<Down>]\<^sub>t (if (if_Some (\<lambda>res. (a,f) \<in> get_valid_locs res) \<omega>_def) then Val v else VFailure)"
 | RedFieldNullFailure:
-   "\<lbrakk> Pr, ctxt, \<omega>_def \<turnstile> \<langle>e; \<omega>\<rangle> [\<Down>]\<^sub>t Val (VRef Null) \<rbrakk> \<Longrightarrow> 
-       Pr, ctxt, \<omega>_def \<turnstile> \<langle>FieldAcc e f; \<omega>\<rangle> [\<Down>]\<^sub>t VFailure"
+   "\<lbrakk> ctxt, R, \<omega>_def \<turnstile> \<langle>e; \<omega>\<rangle> [\<Down>]\<^sub>t Val (VRef Null) \<rbrakk> \<Longrightarrow> 
+       ctxt, R, \<omega>_def \<turnstile> \<langle>FieldAcc e f; \<omega>\<rangle> [\<Down>]\<^sub>t VFailure"
 
 \<comment>\<open>Function application\<close>
-| RedFunApp: "\<lbrakk> (fun_interp_total ctxt) fname = Some f;
-                red_pure_exps_total Pr ctxt \<omega>_def es \<omega> (Some vs);                
-                f vs \<omega> = Some res \<rbrakk> \<Longrightarrow> 
-                Pr, ctxt, \<omega>_def \<turnstile> \<langle>FunApp fname es; \<omega>\<rangle> [\<Down>]\<^sub>t res"
+| RedFunApp: (* Should function application be expression via an operational view? *)
+   "\<lbrakk> (fun_interp_total ctxt) fname = Some f;
+      red_pure_exps_total ctxt R \<omega>_def es \<omega> (Some vs);                
+      f vs \<omega> = Some res \<rbrakk> \<Longrightarrow> 
+      ctxt, R, \<omega>_def \<turnstile> \<langle>FunApp fname es; \<omega>\<rangle> [\<Down>]\<^sub>t res"
 
 \<comment>\<open>Permission introspection\<close>
-| RedPermNull: "\<lbrakk> Pr, ctxt, \<omega>_def \<turnstile> \<langle>e; \<omega>\<rangle> [\<Down>]\<^sub>t Val (VRef Null) \<rbrakk> \<Longrightarrow> Pr, ctxt, \<omega>_def \<turnstile> \<langle>Perm e f; \<omega>\<rangle> [\<Down>]\<^sub>t Val (VPerm 0)"
-| RedPerm: "\<lbrakk> Pr, ctxt, \<omega>_def \<turnstile> \<langle>e; \<omega>\<rangle> [\<Down>]\<^sub>t Val (VRef (Address a));
-              get_mh_total_full \<omega> (a, f) = v \<rbrakk> \<Longrightarrow> 
-             Pr, ctxt, \<omega>_def \<turnstile> \<langle>Perm e f; \<omega>\<rangle> [\<Down>]\<^sub>t Val (VPerm (Rep_prat v))"
+| RedPermNull: (* TODO: should perm(null.f) reduce to failure? *)
+    "\<lbrakk> ctxt, R, \<omega>_def \<turnstile> \<langle>e; \<omega>\<rangle> [\<Down>]\<^sub>t Val (VRef Null) \<rbrakk> \<Longrightarrow> 
+     ctxt, R, \<omega>_def \<turnstile> \<langle>Perm e f; \<omega>\<rangle> [\<Down>]\<^sub>t Val (VPerm 0)"
+| RedPerm: 
+   "\<lbrakk> ctxt, R, \<omega>_def \<turnstile> \<langle>e; \<omega>\<rangle> [\<Down>]\<^sub>t Val (VRef (Address a));
+      get_mh_total_full \<omega> (a, f) = v \<rbrakk> \<Longrightarrow> 
+      ctxt, R, \<omega>_def \<turnstile> \<langle>Perm e f; \<omega>\<rangle> [\<Down>]\<^sub>t Val (VPerm (Rep_prat v))"
 
 \<comment>\<open>Unfolding\<close>
-(* TODO: currently unfolding rules only make sense for inductive predicates, since each recursive unfolding instance is checked *)
-| RedUnfolding: "\<lbrakk> Pr, ctxt, None \<turnstile> \<langle>ubody; \<omega>\<rangle> [\<Down>]\<^sub>t v \<rbrakk> \<Longrightarrow>   
-     Pr, ctxt, None \<turnstile> \<langle>Unfolding p es ubody; \<omega>\<rangle> [\<Down>]\<^sub>t v"
+| RedUnfolding: "\<lbrakk> ctxt, R, None \<turnstile> \<langle>ubody; \<omega>\<rangle> [\<Down>]\<^sub>t v \<rbrakk> \<Longrightarrow>   
+     ctxt, R, None \<turnstile> \<langle>Unfolding p es ubody; \<omega>\<rangle> [\<Down>]\<^sub>t v"
 | RedUnfoldingDef: 
-   "\<lbrakk> red_pure_exps_total Pr ctxt (Some \<omega>_def) es \<omega> (Some vs);
-     unfold_rel Pr ctxt p vs pwrite \<omega>_def \<omega>'_def; 
-     Pr, ctxt, (Some \<omega>'_def) \<turnstile> \<langle>ubody; \<omega>\<rangle> [\<Down>]\<^sub>t v \<rbrakk> \<Longrightarrow>   
-     Pr, ctxt, (Some \<omega>_def) \<turnstile> \<langle>Unfolding p es ubody ; \<omega>\<rangle> [\<Down>]\<^sub>t v"
+   "\<lbrakk> red_pure_exps_total ctxt R (Some \<omega>_def) es \<omega> (Some vs);
+     unfold_rel ctxt R p vs pwrite \<omega>_def \<omega>'_def; 
+     ctxt, R, (Some \<omega>'_def) \<turnstile> \<langle>ubody; \<omega>\<rangle> [\<Down>]\<^sub>t v \<rbrakk> \<Longrightarrow>   
+     ctxt, R, (Some \<omega>_def) \<turnstile> \<langle>Unfolding p es ubody ; \<omega>\<rangle> [\<Down>]\<^sub>t v"
 
-\<comment>\<open>sub_pure_exp currently includes the body of \<open>Unfolding\<close> which is incorrect here\<close>
-| RedSubFailure: "\<lbrakk> e \<in> sub_pure_exp_total e' ; Pr, ctxt, \<omega>_def \<turnstile> \<langle>e; \<omega>\<rangle> [\<Down>]\<^sub>t VFailure \<rbrakk> \<Longrightarrow> 
-     Pr, ctxt, \<omega>_def \<turnstile> \<langle>e'; \<omega>\<rangle> [\<Down>]\<^sub>t VFailure"
-(* Pure quantifier rules (ignore for now)
-(* todo fix interpretation in set_from_type *)
-| RedForallTrue: "\<lbrakk> \<And>v. v \<in> set_from_type f ty \<longrightarrow> Pr, ctxt, \<omega>_def \<turnstile> \<langle>e; shift_and_add_state \<omega> v\<rangle> [\<Down>]\<^sub>t Val (VBool True) \<rbrakk> \<Longrightarrow> 
-     Pr, ctxt, \<omega>_def \<turnstile> \<langle>PForall ty e; \<omega>\<rangle> [\<Down>]\<^sub>t Val (VBool True)"
-| RedForallFalse: "\<lbrakk> v \<in> set_from_type f ty ; Pr, ctxt, \<omega>_def \<turnstile> \<langle>e; shift_and_add_state \<omega> v\<rangle> [\<Down>]\<^sub>t Val (VBool False) \<rbrakk>
-  \<Longrightarrow> Pr, ctxt, \<omega>_def \<turnstile> \<langle>PForall ty e; \<omega>\<rangle> [\<Down>]\<^sub>t Val (VBool False)"
-(* not clear if one wants to avoid that forall can reduce to false and failure in the same state *)
-| RedForallFailure:  "\<lbrakk> v \<in> set_from_type f ty ; Pr, ctxt, \<omega>_def \<turnstile> \<langle>e; shift_and_add_state \<omega> v\<rangle> [\<Down>]\<^sub>t VFailure \<rbrakk>
-  \<Longrightarrow> Pr, ctxt, \<omega>_def \<turnstile> \<langle>PForall ty e; \<omega>\<rangle> [\<Down>]\<^sub>t VFailure"
-
-(* todo fix interpretation in set_from_type *)
-| RedExistsTrue: "\<lbrakk> v \<in> set_from_type f ty ; Pr, ctxt, \<omega>_def \<turnstile> \<langle>e; shift_and_add_state \<omega> v\<rangle> [\<Down>]\<^sub>t Val (VBool True) \<rbrakk> \<Longrightarrow>
-  Pr, ctxt, \<omega>_def \<turnstile> \<langle>PExists ty e; \<omega>\<rangle> [\<Down>]\<^sub>t Val (VBool True)"
-(* not clear if one wants to avoid that forall can reduce to true and failure in the same state *)
-| RedExistsFalse: "\<lbrakk> \<And> v. v \<in> set_from_type f ty \<Longrightarrow> Pr, ctxt, \<omega>_def \<turnstile> \<langle>e; shift_and_add_state \<omega> v\<rangle> [\<Down>]\<^sub>t Val (VBool False) \<rbrakk> \<Longrightarrow>
-  Pr, ctxt, \<omega>_def \<turnstile> \<langle>PExists ty e; \<omega>\<rangle> [\<Down>]\<^sub>t Val (VBool True)"
-| RedExistsFailure: "\<lbrakk>v \<in> set_from_type f ty ; Pr, ctxt, \<omega>_def \<turnstile> \<langle>e; shift_and_add_state \<omega> v\<rangle> [\<Down>]\<^sub>t VFailure \<rbrakk> \<Longrightarrow>
-  Pr, ctxt, \<omega>_def \<turnstile> \<langle>PExists ty e; \<omega>\<rangle> [\<Down>]\<^sub>t VFailure"
-*)
-(*
-| RedForallFalse: "\<lbrakk> v \<in> set_from_type ctxt ty ; Pr, ctxt \<turnstile> \<langle>e; shift_and_add_state \<omega> v\<rangle> [\<Down>]\<^sub>t Val (VBool False) \<rbrakk>
-  \<Longrightarrow> Pr, ctxt \<turnstile> \<langle>PForall ty e; \<omega>\<rangle> [\<Down>]\<^sub>t Val (VBool False)"*)
-
-(*
-(* perm(P(...)) = 0 if equirecursive *)
-| RedPermPred: "\<lbrakk> list_all2 (\<lambda>e v. Pr, ctxt \<turnstile> \<langle>e; \<omega>\<rangle> [\<Down>] Val v) exps vals \<rbrakk>
-  \<Longrightarrow> Pr, ctxt \<turnstile> \<langle>PermPred p exps; \<omega>\<rangle> [\<Down>] Val (VPerm (Rep_prat (get_pm \<omega> (p, vals))))"
-*)
-(*| RedLet: "\<lbrakk> Pr, ctxt \<turnstile> \<langle>e1; \<omega>\<rangle> [\<Down>]\<^sub>t Val v1 ; Pr, ctxt \<turnstile> \<langle>e2; shift_and_add_state \<omega> v1\<rangle> [\<Down>]\<^sub>t r \<rbrakk> \<Longrightarrow> Pr, ctxt \<turnstile> \<langle>Let e1 e2; \<omega>\<rangle> [\<Down>]\<^sub>t r" *)
+\<comment>\<open>Important: \<^const>\<open>sub_pure_exp_total\<close> should not include the body of an unfolding\<close>
+| RedSubFailure: "\<lbrakk> e \<in> sub_pure_exp_total e' ; ctxt, R, \<omega>_def \<turnstile> \<langle>e; \<omega>\<rangle> [\<Down>]\<^sub>t VFailure \<rbrakk> \<Longrightarrow> 
+     ctxt, R, \<omega>_def \<turnstile> \<langle>e'; \<omega>\<rangle> [\<Down>]\<^sub>t VFailure"
 
 thm red_pure_exp_total_red_pure_exps_total_red_inhale_unfold_rel.induct
-(*
-lemma red_total_with_wf_implies_without_wf:
-  assumes "Pr, ctxt_vpr, Some \<omega>' \<turnstile> \<langle>e_vpr; \<omega>\<rangle> [\<Down>]\<^sub>t Val v1 \<Longrightarrow> Pr, ctxt_vpr, None \<turnstile> \<langle>e_vpr; \<omega>\<rangle> [\<Down>]\<^sub>t Val v1" and
-          "red_pure_exps_total Pr ctxt Some \<omega>' es \<omega> (Some vs) \<Longrightarrow> red_pure_exps_total Pr ctxt None \<omega>' es \<omega> (Some vs)"
-*)
 
 subsubsection \<open>Elimination rules\<close>
 
@@ -343,79 +340,22 @@ inductive_cases RedPerm_case: "Pr, ctxt, \<omega>_def \<turnstile> \<langle>Perm
 
 lemmas red_pure_exp_total_elims = RedUnop_case RedBinop_case RedFunApp_case RedExpList_case
 
-subsection \<open>Simplified induction principles\<close>
-lemma conj2conj2: "A \<and> B \<and> C \<Longrightarrow> C"
-  apply (drule conjunct2)
-  apply (drule conjunct2)
-  by assumption
-
-lemma conj2conj2conj1: "A \<and> B \<and> C \<and> D \<Longrightarrow> C"
-  apply (drule conjunct2)
-  apply (drule conjunct2)
-  apply (drule conjunct1)
-  by assumption
-
-
-lemmas red_inhale_induct_aux = mp[OF conj2conj2conj1[OF 
-      red_pure_exp_total_red_pure_exps_total_red_inhale_unfold_rel.induct[where ?P1.0 = "\<lambda> a b c d. True" and ?P2.0 = "\<lambda> a b c d. True" and ?P4.0 = "\<lambda> a b c d e. True"]]]
-
-lemma red_inhale_induct [consumes 1, case_names InhAcc InhAccPred InhAccWildcard InhAccPredWildcard 
-InhPureNormalMagic InhSubFailure InhSepNormal InhSepFailureMagic InhImpTrue InhImpFalse InhImpFailure]:
-  assumes "red_inhale Pr ctxt R A \<omega> res" and
-    "(\<And>\<omega> e_r r e_p p W' R f res.
-            Pr, ctxt, (Some \<omega>) \<turnstile> \<langle>e_r;\<omega>\<rangle> [\<Down>]\<^sub>t Val (VRef r) \<Longrightarrow>
-            Pr, ctxt, (Some \<omega>) \<turnstile> \<langle>e_p;\<omega>\<rangle> [\<Down>]\<^sub>t Val (VPerm p) \<Longrightarrow>
-            W' = inhale_perm_single R \<omega> (the_address r, f) (Some (Abs_prat p)) \<Longrightarrow>
-            th_result_rel (0 \<le> p) (W' \<noteq> {} \<and> r \<noteq> Null) W' res \<Longrightarrow> P R (Atomic (Acc e_r f (PureExp e_p))) \<omega> res)" and
-    "(\<And>\<omega> e_p p e_args v_args W' R pred_id res.
-            Pr, ctxt, (Some \<omega>) \<turnstile> \<langle>e_p;\<omega>\<rangle> [\<Down>]\<^sub>t Val (VPerm p) \<Longrightarrow>
-            red_pure_exps_total Pr ctxt (Some \<omega>) e_args \<omega> (Some v_args) \<Longrightarrow>
-            W' = inhale_perm_single_pred R \<omega> (pred_id, v_args) (Some (Abs_prat p)) \<Longrightarrow>
-            th_result_rel (0 \<le> p) (W' \<noteq> {}) W' res \<Longrightarrow> P R (Atomic (AccPredicate pred_id e_args (PureExp e_p))) \<omega> res)" and
-    "(\<And>\<omega> e_r r W' R f res.
-            Pr, ctxt, (Some \<omega>) \<turnstile> \<langle>e_r;\<omega>\<rangle> [\<Down>]\<^sub>t Val (VRef r) \<Longrightarrow>
-            W' = inhale_perm_single R \<omega> (the_address r, f) None \<Longrightarrow>
-            th_result_rel True (W' \<noteq> {} \<and> r \<noteq> Null) W' res \<Longrightarrow> P R (Atomic (Acc e_r f Wildcard)) \<omega> res)" and
-    "(\<And>\<omega> e_args v_args W' R pred_id res.
-            red_pure_exps_total Pr ctxt (Some \<omega>) e_args \<omega> (Some v_args) \<Longrightarrow>
-            W' = inhale_perm_single_pred R \<omega> (pred_id, v_args) None \<Longrightarrow>
-            th_result_rel True (W' \<noteq> {}) W' res \<Longrightarrow> P R (Atomic (AccPredicate pred_id e_args Wildcard)) \<omega> res)"
-    "(\<And>\<omega> e b R.
-            Pr, ctxt, (Some \<omega>) \<turnstile> \<langle>e;\<omega>\<rangle> [\<Down>]\<^sub>t Val (VBool b) \<Longrightarrow>
-            P R (Atomic (Pure e)) \<omega> (if b then RNormal \<omega> else RMagic))" and
-    "(\<And>e A \<omega> R.
-            e \<in> sub_expressions_atomic A \<Longrightarrow> Pr, ctxt, (Some \<omega>) \<turnstile> \<langle>e;\<omega>\<rangle> [\<Down>]\<^sub>t VFailure \<Longrightarrow> True \<Longrightarrow> P R (Atomic A) \<omega> RFailure)" and
-    "(\<And>R A \<omega> \<omega>'' B res.
-            red_inhale Pr ctxt R A \<omega> (RNormal \<omega>'') \<Longrightarrow>
-            P R A \<omega> (RNormal \<omega>'') \<Longrightarrow> red_inhale Pr ctxt R B \<omega>'' res \<Longrightarrow> P R B \<omega>'' res \<Longrightarrow> P R (A && B) \<omega> res)" and
-    "(\<And>R A \<omega> resA B. red_inhale Pr ctxt R A \<omega> resA \<Longrightarrow> P R A \<omega> resA \<Longrightarrow> resA = RFailure \<or> resA = RMagic \<Longrightarrow> P R (A && B) \<omega> resA)" and
-    "(\<And>\<omega> e R A res.
-            Pr, ctxt, (Some \<omega>) \<turnstile> \<langle>e;\<omega>\<rangle> [\<Down>]\<^sub>t Val (VBool True) \<Longrightarrow>
-            red_inhale Pr ctxt R A \<omega> res \<Longrightarrow> P R A \<omega> res \<Longrightarrow> P R (Imp e A) \<omega> res)" and
-    "(\<And>\<omega> e R A. Pr, ctxt, (Some \<omega>) \<turnstile> \<langle>e;\<omega>\<rangle> [\<Down>]\<^sub>t Val (VBool False) \<Longrightarrow> P R (Imp e A) \<omega> (RNormal \<omega>))" and
-    "(\<And>\<omega> e R A. Pr, ctxt, (Some \<omega>) \<turnstile> \<langle>e;\<omega>\<rangle> [\<Down>]\<^sub>t VFailure \<Longrightarrow> P R (Imp e A) \<omega> RFailure)" and
-    "(\<And>\<omega> e R A. Pr, ctxt, (Some \<omega>) \<turnstile> \<langle>e;\<omega>\<rangle> [\<Down>]\<^sub>t VFailure \<Longrightarrow> P R (Imp e A) \<omega> RFailure)"
- shows "P R A \<omega> res"
-  apply (rule red_inhale_induct_aux[where ?P3.0=P])
-  apply simp
-  by (tactic \<open>resolve_tac @{context} @{thms assms} 1\<close>, assumption+)+ (auto intro: assms(1))
-
 subsection \<open>Total heap consistency\<close>
 
-definition unfold_rel_general :: "program \<Rightarrow> 'a total_context \<Rightarrow> 'a full_total_state \<Rightarrow> 'a full_total_state \<Rightarrow> bool"
-  where "unfold_rel_general Pr ctxt \<omega> \<omega>' \<equiv> \<exists> pred_id vs q. unfold_rel Pr ctxt pred_id vs q \<omega> \<omega>'"
+definition unfold_rel_general :: "'a total_context \<Rightarrow> ('a full_total_state \<Rightarrow> bool) \<Rightarrow> 'a full_total_state \<Rightarrow> 'a full_total_state \<Rightarrow> bool"
+  where "unfold_rel_general ctxt R \<omega> \<omega>' \<equiv> \<exists> pred_id vs q. unfold_rel ctxt R pred_id vs q \<omega> \<omega>'"
 
-definition unfold_rel_multi :: "program \<Rightarrow> 'a total_context \<Rightarrow> 'a full_total_state \<Rightarrow> 'a full_total_state \<Rightarrow> bool"
-  where "unfold_rel_multi Pr ctxt  \<equiv> rtranclp (unfold_rel_general Pr ctxt)"
+definition unfold_rel_multi :: "'a total_context \<Rightarrow> ('a full_total_state \<Rightarrow> bool) \<Rightarrow>'a full_total_state \<Rightarrow> 'a full_total_state \<Rightarrow> bool"
+  where "unfold_rel_multi ctxt R  \<equiv> rtranclp (unfold_rel_general ctxt R)"
 
 text \<open>Expression evaluation as a function. Using this function makes sense, when it is known that 
 e is well-defined and is deterministic (for example, if e is the body of a predicate).\<close>
 
-fun red_pure_exp_total_fun :: "program \<Rightarrow> 'a total_context \<Rightarrow> pure_exp \<Rightarrow> 'a full_total_state \<Rightarrow> 'a val"
-  where "red_pure_exp_total_fun Pr ctxt e \<omega> = (SOME v. Pr, ctxt, None \<turnstile> \<langle>e; \<omega>\<rangle> [\<Down>]\<^sub>t Val v)"
+fun red_pure_exp_total_fun :: "'a total_context \<Rightarrow> pure_exp \<Rightarrow> 'a full_total_state \<Rightarrow> 'a val"
+  where "red_pure_exp_total_fun ctxt e \<omega> = (SOME v. ctxt, (\<lambda>_. True), None \<turnstile> \<langle>e; \<omega>\<rangle> [\<Down>]\<^sub>t Val v)"
 
-fun red_pure_exps_total_fun :: "program \<Rightarrow> 'a total_context \<Rightarrow> pure_exp list \<Rightarrow> 'a full_total_state \<Rightarrow> ('a val) list"
-  where "red_pure_exps_total_fun Pr ctxt es \<omega> = (SOME vs. red_pure_exps_total Pr ctxt None es \<omega> (Some vs))"
+fun red_pure_exps_total_fun :: "'a total_context \<Rightarrow> pure_exp list \<Rightarrow> 'a full_total_state \<Rightarrow> ('a val) list"
+  where "red_pure_exps_total_fun ctxt es \<omega> = (SOME vs. red_pure_exps_total ctxt (\<lambda>_. True)  None es \<omega> (Some vs))"
 
 (* TODO: duplicate? *)
 fun extract_address_from_val :: "'a val \<Rightarrow> address"
@@ -429,78 +369,84 @@ fun extract_perm_from_val :: "'a val \<Rightarrow> rat"
     "extract_perm_from_val (VPerm r) = r"
   | "extract_perm_from_val _ = undefined"
 
-fun is_positive_permission :: "program \<Rightarrow> 'a total_context \<Rightarrow> pure_exp exp_or_wildcard \<Rightarrow> 'a full_total_state \<Rightarrow> bool"
+fun is_positive_permission :: "'a total_context \<Rightarrow> pure_exp exp_or_wildcard \<Rightarrow> 'a full_total_state \<Rightarrow> bool"
   where 
-    "is_positive_permission Pr ctxt Wildcard \<omega> = True"
-  | "is_positive_permission Pr ctxt (PureExp e) \<omega> = (extract_perm_from_val (red_pure_exp_total_fun Pr ctxt e \<omega>) > 0)"
+    "is_positive_permission ctxt Wildcard \<omega> = True"
+  | "is_positive_permission ctxt (PureExp e) \<omega> = (extract_perm_from_val (red_pure_exp_total_fun ctxt e \<omega>) > 0)"
 
 
-fun assertion_heap_snapshot :: "program \<Rightarrow> 'a total_context \<Rightarrow> assertion \<Rightarrow> 'a full_total_state \<Rightarrow> heap_loc set"
+fun assertion_heap_snapshot :: "'a total_context \<Rightarrow> assertion \<Rightarrow> 'a full_total_state \<Rightarrow> heap_loc set"
   where 
-   "assertion_heap_snapshot Pr ctxt (Atomic (Pure e)) \<omega> = {}"
- | "assertion_heap_snapshot Pr ctxt (Atomic (Acc e f e_p)) \<omega> = 
-             (if is_positive_permission Pr ctxt e_p \<omega> then 
-                  {(extract_address_from_val (red_pure_exp_total_fun Pr ctxt e \<omega>), f)} 
+   "assertion_heap_snapshot ctxt (Atomic (Pure e)) \<omega> = {}"
+ | "assertion_heap_snapshot ctxt (Atomic (Acc e f e_p)) \<omega> = 
+             (if is_positive_permission ctxt e_p \<omega> then 
+                  {(extract_address_from_val (red_pure_exp_total_fun ctxt e \<omega>), f)} 
               else {})"
- | "assertion_heap_snapshot Pr ctxt (Atomic (AccPredicate pred_id e_args e_p)) \<omega> = 
-             (if is_positive_permission Pr ctxt e_p \<omega> then
-                fst (get_hp_total_full \<omega> (pred_id, red_pure_exps_total_fun Pr ctxt e_args \<omega>))
+ | "assertion_heap_snapshot ctxt (Atomic (AccPredicate pred_id e_args e_p)) \<omega> = 
+             (if is_positive_permission ctxt e_p \<omega> then
+                fst (get_hp_total_full \<omega> (pred_id, red_pure_exps_total_fun ctxt e_args \<omega>))
               else {})"
- | "assertion_heap_snapshot Pr ctxt (Imp e A) \<omega> =
-             (if red_pure_exp_total_fun Pr ctxt e \<omega> = VBool True then 
-                 assertion_heap_snapshot Pr ctxt A \<omega> 
+ | "assertion_heap_snapshot ctxt (Imp e A) \<omega> =
+             (if red_pure_exp_total_fun ctxt e \<omega> = VBool True then 
+                 assertion_heap_snapshot ctxt A \<omega> 
               else {})"
- | "assertion_heap_snapshot Pr ctxt (A && B) \<omega> = assertion_heap_snapshot Pr ctxt A \<omega> \<union> assertion_heap_snapshot Pr ctxt B \<omega>"      
- | "assertion_heap_snapshot Pr ctxt _ \<omega> = undefined" (* wands and quantified permissions not supported *)
+ | "assertion_heap_snapshot ctxt (A && B) \<omega> = assertion_heap_snapshot ctxt A \<omega> \<union> assertion_heap_snapshot ctxt B \<omega>"      
+ | "assertion_heap_snapshot ctxt _ \<omega> = undefined" (* wands and quantified permissions not supported *)
 
-fun assertion_predicate_snapshot :: "program \<Rightarrow> 'a total_context \<Rightarrow> assertion \<Rightarrow> 'a full_total_state \<Rightarrow> 'a predicate_loc set"
+fun assertion_predicate_snapshot :: "'a total_context \<Rightarrow> assertion \<Rightarrow> 'a full_total_state \<Rightarrow> 'a predicate_loc set"
   where 
-   "assertion_predicate_snapshot Pr ctxt (Atomic (Pure e)) \<omega> = {}"
- | "assertion_predicate_snapshot Pr ctxt (Atomic (Acc e f e_p)) \<omega> = {}"
- | "assertion_predicate_snapshot Pr ctxt (Atomic (AccPredicate pred_id e_args e_p)) \<omega> = 
-             (if is_positive_permission Pr ctxt e_p \<omega> then
-                {(pred_id, red_pure_exps_total_fun Pr ctxt e_args \<omega>)} \<union> 
-                snd (get_hp_total_full \<omega> (pred_id, red_pure_exps_total_fun Pr ctxt e_args \<omega>))
+   "assertion_predicate_snapshot ctxt (Atomic (Pure e)) \<omega> = {}"
+ | "assertion_predicate_snapshot ctxt (Atomic (Acc e f e_p)) \<omega> = {}"
+ | "assertion_predicate_snapshot ctxt (Atomic (AccPredicate pred_id e_args e_p)) \<omega> = 
+             (if is_positive_permission ctxt e_p \<omega> then
+                {(pred_id, red_pure_exps_total_fun ctxt e_args \<omega>)} \<union> 
+                snd (get_hp_total_full \<omega> (pred_id, red_pure_exps_total_fun ctxt e_args \<omega>))
               else {})"
- | "assertion_predicate_snapshot Pr ctxt (Imp e A) \<omega> =
-             (if red_pure_exp_total_fun Pr ctxt e \<omega> = VBool True then 
-                 assertion_predicate_snapshot Pr ctxt A \<omega> 
+ | "assertion_predicate_snapshot ctxt (Imp e A) \<omega> =
+             (if red_pure_exp_total_fun ctxt e \<omega> = VBool True then 
+                 assertion_predicate_snapshot ctxt A \<omega> 
               else {})"
- | "assertion_predicate_snapshot Pr ctxt (A && B) \<omega> = assertion_predicate_snapshot Pr ctxt A \<omega> \<union> assertion_predicate_snapshot Pr ctxt B \<omega>"      
- | "assertion_predicate_snapshot Pr ctxt _ \<omega> = undefined" (* wands and quantified permissions not supported *)
+ | "assertion_predicate_snapshot ctxt (A && B) \<omega> = assertion_predicate_snapshot ctxt A \<omega> \<union> assertion_predicate_snapshot ctxt B \<omega>"      
+ | "assertion_predicate_snapshot ctxt _ \<omega> = undefined" (* wands and quantified permissions not supported *)
 
 
-definition pheap_consistent :: "program \<Rightarrow> 'a total_context \<Rightarrow> 'a full_total_state \<Rightarrow> bool" where
- "pheap_consistent Pr ctxt \<omega> \<equiv> 
-    \<forall> \<omega>' pred_id vs pred_decl. 
-         (pgt (get_mp_total_full \<omega>' (pred_id,vs)) pnone \<and> ViperLang.predicates Pr pred_id = Some pred_decl) \<longrightarrow>
+(* TODO: Should the state track the predicate heap explicitly? *)
+definition pheap_consistent :: "'a total_context \<Rightarrow> 'a full_total_state \<Rightarrow> bool" where
+ "pheap_consistent ctxt \<omega> \<equiv> 
+    \<forall> pred_id vs pred_decl. 
+         (pgt (get_mp_total_full \<omega> (pred_id,vs)) pnone \<and> ViperLang.predicates (program_total ctxt) pred_id = Some pred_decl) \<longrightarrow>
           option_fold (\<lambda> pred_body. get_hp_total_full \<omega> (pred_id, vs) = 
-                        (assertion_heap_snapshot Pr ctxt pred_body (update_store_total \<omega> (nth_option vs)), assertion_predicate_snapshot Pr ctxt pred_body (update_store_total \<omega> (nth_option vs))) )
+                        (assertion_heap_snapshot ctxt pred_body (update_store_total \<omega> (nth_option vs)), assertion_predicate_snapshot ctxt pred_body (update_store_total \<omega> (nth_option vs))) )
                       True
                       (ViperLang.predicate_decl.body pred_decl)"
 
-(* TODO: for infinite predciates pheap consistent allows larger predicate heaps than necessary *)
-
-coinductive total_heap_consistent :: "program \<Rightarrow> 'a total_context \<Rightarrow> 'a full_total_state \<Rightarrow> bool"
-  for Pr :: program and ctxt :: "'a total_context"
+inductive total_heap_consistent :: "'a total_context \<Rightarrow> 'a full_total_state \<Rightarrow> bool"
+  for ctxt :: "'a total_context"
   where 
-  UnfoldStep: "\<lbrakk> \<And> pred_id vs q.                      
-                     option_fold (\<lambda>decl. ViperLang.predicate_decl.body decl) None (ViperLang.predicates Pr pred_id) \<noteq> None \<Longrightarrow>
-                     pgte (get_mp_total_full \<omega> (pred_id,vs)) q \<and> q \<noteq> pnone  \<Longrightarrow>
-                     \<exists>\<omega>'. unfold_rel Pr ctxt pred_id vs q \<omega> \<omega>' \<and> total_heap_consistent Pr ctxt \<omega>';
-                 pheap_consistent Pr ctxt \<omega> \<rbrakk> \<Longrightarrow>
-                 total_heap_consistent Pr ctxt \<omega>"
+  \<comment>\<open>If a state does contain any permission to non-abstract predicates, then the state is trivially consistent.\<close>
+  ConsistentNoPred: 
+  " \<lbrakk> \<And> pred_id vs. option_fold (\<lambda>decl. ViperLang.predicate_decl.body decl) None (ViperLang.predicates (program_total ctxt) pred_id) \<noteq> None \<Longrightarrow>
+                    get_mp_total_full \<omega> (pred_id,vs) = pnone \<rbrakk> \<Longrightarrow> 
+                    total_heap_consistent ctxt \<omega>"
+  \<comment>\<open>If a state contains permission to a non-abstract predicate, then the state is consistent if some such non-abstract predicate
+     can be completely unfolded to reach another consistent state\<close>
+| UnfoldStep: "\<lbrakk> option_fold (\<lambda>decl. ViperLang.predicate_decl.body decl) None (ViperLang.predicates (program_total ctxt) pred_id) \<noteq> None;
+                 q = (get_mp_total_full \<omega> (pred_id,vs));
+                 pgt p pnone;
+                 \<exists>\<omega>'. unfold_rel ctxt (\<lambda>_. True) pred_id vs q \<omega> \<omega>' \<and> total_heap_consistent ctxt \<omega>';
+                 pheap_consistent ctxt \<omega> \<rbrakk> \<Longrightarrow>
+                 total_heap_consistent ctxt \<omega>"
 
 
-abbreviation red_inhale_th_cons :: "program \<Rightarrow> 'a total_context \<Rightarrow> assertion \<Rightarrow> 'a full_total_state \<Rightarrow> 'a standard_result \<Rightarrow> bool"
-  where "red_inhale_th_cons Pr ctxt A \<omega> res \<equiv> red_inhale Pr ctxt (total_heap_consistent Pr ctxt) A \<omega> res"
+abbreviation red_inhale_th_cons :: "'a total_context \<Rightarrow> assertion \<Rightarrow> 'a full_total_state \<Rightarrow> 'a standard_result \<Rightarrow> bool"
+  where "red_inhale_th_cons ctxt A \<omega> res \<equiv> red_inhale ctxt (total_heap_consistent ctxt) A \<omega> res"
 
 text \<open>\<^const>\<open>red_inhale_th_cons\<close> only takes transitions to total heap consistent states whenever some 
 permission is inhaled\<close>
 
-definition assertion_self_framing_store :: "program \<Rightarrow> 'a total_context \<Rightarrow> assertion \<Rightarrow> 'a store \<Rightarrow> bool"
+definition assertion_self_framing_store :: "'a total_context \<Rightarrow> assertion \<Rightarrow> 'a store \<Rightarrow> bool"
   where
-    "assertion_self_framing_store Pr ctxt A \<sigma> = (\<forall> \<omega> res. red_inhale_th_cons Pr ctxt A (update_store_total \<omega> \<sigma>) res \<longrightarrow> res \<noteq> RFailure)"
-
+    "assertion_self_framing_store ctxt A \<sigma> \<equiv> 
+      \<forall> \<omega> res. red_inhale_th_cons ctxt A (update_store_total \<omega> \<sigma>) res \<longrightarrow> res \<noteq> RFailure"
 
 end
